small-step and large-step semantics

LeanLgtm/Basic.lean
@@ -1,6 +1,7 @@
 import Ssreflect.Lang
+import Mathlib.Data.Finmap
 
-
+/- -------- Language Syntax -------------------------- -/
 /-
 Inductive prim : Type :=
   | val_ref : prim
@@ -49,24 +50,480 @@ abbrev var := String
 
 def null : loc := 0
 
+mutual
+  inductive val : Type where
+    | val_unit : val
+    | val_bool : Bool → val
+    | val_int : Int → val
+    | val_loc : loc → val
+    | val_prim : prim → val
+    | val_fun : var -> trm -> val
+    | val_fix : var -> var -> trm -> val
+    | val_uninit : val
+    | val_error : val
 
-inductive val where
-  | val_unit : val
-  | val_bool : Bool → val
-  | val_int : Int → val
-  | val_loc : loc → val
-  | val_prim : prim → val
-  | val_fun : var -> trm -> val
-  | val_fiv : var -> var -> trm -> val
-  | val_uninit : val
-  | val_error : val
-  with
-inductive trm where
-  | trm_val : val -> trm
-  | trm_var : var -> trm
-  | trm_fun : var -> trm -> trm
-  | trm_fix : var -> var -> trm -> trm
-  | trm_app : trm -> trm -> trm
-  | trm_seq : trm -> trm -> trm
-  | trm_let : var -> trm -> trm -> trm
-  | trm_if : trm -> trm -> trm -> trm
+  inductive trm : Type where
+    | trm_val : val -> trm
+    | trm_var : var -> trm
+    | trm_fun : var -> trm -> trm
+    | trm_fix : var -> var -> trm -> trm
+    | trm_app : trm -> trm -> trm
+    | trm_seq : trm -> trm -> trm
+    | trm_let : var -> trm -> trm -> trm
+    | trm_if : trm -> trm -> trm -> trm
+end
+
+/- States and heaps are represented as finite maps -/
+abbrev state := Finmap (λ _ : loc ↦ val)
+abbrev heap := state
+
+
+/- ---------------- Notations ----------------- -/
+/- Declaring implicit types for meta-variables -/
+variable (f : var)
+variable (b : Bool)
+variable (p : loc)
+variable (n : Int)
+variable (v w r vf vx : val)
+variable (t : trm)
+variable (h : heap)
+variable (s : state)
+
+/- val and term are inhabited -/
+instance : Inhabited val where
+  default := val.val_unit
+
+instance : Inhabited trm where
+  default := trm.trm_val (val.val_unit)
+
+/- Coercions -/
+instance : Coe Bool val where
+  coe b := val.val_bool b
+
+instance : Coe Int val where
+  coe z := val.val_int z
+
+instance : Coe loc val where
+  coe l := val.val_loc l
+
+instance : Coe prim val where
+  coe x := val.val_prim x
+
+instance : Coe val trm where
+  coe v := trm.trm_val v
+
+instance : Coe var trm where
+  coe x := trm.trm_var x
+
+
+/- ------------- Terms, Values and Substitutions -------------- -/
+open trm
+
+def trm_is_val : trm → Prop
+  | trm_val _ => true
+  | _         => false
+
+/- Capture-avoiding substitution -/
+def subst (y : var) (v' : val) (t : trm) : trm :=
+  -- let aux x := subst y v' x
+  let if_y_eq x t1 t2 := if x = y then t1 else t2
+  match t with
+  | trm_val v => trm_val v
+  | trm_var x => if_y_eq x (trm_val v') t
+  | trm_fun x t1 => trm_fun x (if_y_eq x t1 (subst y v' t1))
+  | trm_fix f x t1 => trm_fix f x (if_y_eq f t1 (if_y_eq x t1 (subst y v' t1)))
+  | trm_app t1 t2 => trm_app (subst y v' t1) (subst y v' t2)
+  | trm_seq t1 t2 => trm_seq (subst y v' t1) (subst y v' t2)
+  | trm_let x t1 t2 => trm_let x (subst y v' t1) (if_y_eq x t2 (subst y v' t2))
+  | trm_if t0 t1 t2 => trm_if (subst y v' t0) (subst y v' t1) (subst y v' t2)
+
+
+/- ------------ Small-Step Semantics ----------------- -/
+open val
+open prim
+
+/- Function for reading a memory location (to unwrap the option) -/
+def read_state (p : loc) (h : state) :=
+  match Finmap.lookup p h with
+  | some v => v
+  | none   => default
+
+/- Skipping the small-step semantics for now since they aren't used in the
+   CFML metatheory except for an alternate soundness proof using small-step
+   semantics rather than big-step semantics. Porting the small-step relation
+   to Lean will require a bit more work with coercions and such due to the way
+   that the types prim, val, and trm are defined.  -/
+inductive step : state → trm → state → trm → Prop where
+
+  -- Context Rules
+  | step_seq_ctx : forall s1 s2 t1 t1' t2,
+      step s1 t1 s2 t1' →
+      step s1 (trm_seq t1 t2) s2 (trm_seq t1' t2)
+  | step_let_ctx : forall s1 s2 x t1 t1' t2,
+      step s1 t1 s2 t1' →
+      step s1 (trm_let x t1 t2) s2 (trm_let x t1' t2)
+  | step_app_arg_1 : forall s1 s2 t1 t1' t2,
+      step s1 t1 s2 t1' →
+      step s1 (trm_app t1 t2) s2 (trm_app t1' t2)
+  | step_app_arg2 : forall s1 s2 v1 t2 t2',
+      step s1 t2 s2 t2' →
+      step s1 (trm_app v1 t2) s2 (trm_app v1 t2')
+
+  -- Reduction
+  | step_fun : forall s x t1,
+      step s (trm_fun x t1) s (val_fun x t1)
+  | step_fix : forall s f x t1,
+      step s (trm_fix f x t1) s (val_fix f x t1)
+  | step_app_fun : forall s v1 v2 x t1,
+      v1 = val_fun x t1 →
+      v2 = trm_val v2' →
+      step s (trm_app v1 v2) s (subst x v2' t1)
+  | step_app_fix : forall s v1 v2 f x t1,
+      v1 = val_fix f x t1 →
+      v2 = trm_val v2' →
+      step s (trm_app v1 v2) s (subst x v2' (subst f v1 t1))
+  | step_if : forall s b t1 t2,
+      step s (trm_if (val_bool b) t1 t2) s (if b then t1 else t2)
+  | step_seq : forall s t2 v1,
+      step s (trm_seq v1 t2) s t2
+  | step_let : forall s x t2 v1,
+      v1 = trm_val v1' →
+      step s (trm_let x v1 t2) s (subst x v1' t2)
+
+  -- Unary Operations
+  | step_neg : forall s b,
+      step s (trm_app val_neg (val_bool b)) s (val_bool (¬ b))
+  | step_opp : forall s n,
+      step s (trm_app val_opp (val_int n)) s (val_int (- n))
+  | step_rand : forall s n n1,
+      0 <= n1 ∧ n1 < n →
+      step s (trm_app val_rand (val_int n)) s (val_int n1)
+
+  -- Binary Operations
+  | step_eq_true : forall s v1 v2,
+      v1 = v2 →
+      step s (trm_app (trm_app val_eq v1) v2) s (val_bool true)
+  | step_eq_false : forall s v1 v2,
+      v1 ≠ v2 →
+      step s (trm_app (trm_app val_eq v1) v2) s (val_bool false)
+  | step_neq_true : forall s v1 v2,
+      v1 ≠ v2 →
+      step s (trm_app (trm_app val_neq v1) v2) s (val_bool true)
+  | step_neq_false : forall s v1 v2,
+      v1 ≠ v2 →
+      step s (trm_app (trm_app val_neq v1) v2) s (val_bool false)
+  | step_add : forall s n1 n2,
+      step s (trm_app (trm_app val_add (val_int n1)) (val_int n2)) s
+        (val_int (n1 + n2))
+  | step_sub : forall s n1 n2,
+      step s (trm_app (trm_app val_sub (val_int n1)) (val_int n2)) s
+        (val_int (n1 - n2))
+  | step_mul : forall s n1 n2,
+      step s (trm_app (trm_app val_mul (val_int n1)) (val_int n2)) s
+        (val_int (n1 * n2))
+  | step_div : forall s n1 n2,
+      n2 ≠ 0 →
+      step s (trm_app (trm_app val_div (val_int n1)) (val_int n2)) s
+        (n1 / n2)
+  | step_mod : forall s n1 n2,
+      n2 ≠ 0 →
+      step s (trm_app (trm_app val_mod (val_int n1)) (val_int n2)) s
+        (n1 % n2)
+  | step_le : forall s n1 n2,
+      step s (trm_app (trm_app val_le (val_int n1)) (val_int n2)) s
+        (val_bool (n1 <= n2))
+  | step_lt : forall s n1 n2,
+      step s (trm_app (trm_app val_lt (val_int n1)) (val_int n2)) s
+        (val_bool (n1 < n2))
+  | step_ge : forall s n1 n2,
+      step s (trm_app (trm_app val_ge (val_int n1)) (val_int n2)) s
+        (val_bool (n1 >= n2))
+  | step_gt : forall s n1 n2,
+      step s (trm_app (trm_app val_gt (val_int n1)) (val_int n2)) s
+        (val_bool (n1 > n2))
+  | step_ptr_add : forall s p1 p2 n,
+      (p2:ℤ) = (p1:loc) + n →
+      step s (trm_app (trm_app val_ptr_add (val_loc p1)) (val_int n)) s
+        (val_loc (Int.toNat p2))
+
+  -- Heap Opeartions
+  | step_ref : forall s v p,
+      ¬ p ∈ s →
+      v = trm_val v' →
+      step s (trm_app val_ref v) (Finmap.insert p v' s) (val_loc p)
+  | step_get : forall s p,
+      p ∈ s →
+      step s (trm_app val_get (val_loc p)) s (read_state p s)
+  | step_set : forall s p v,
+      p ∈ s ->
+      v = trm_val v' →
+      step s (trm_app (trm_app val_set (val_loc p)) v)
+        (Finmap.insert p v' s) val_unit
+  | step_free : forall s p,
+      p ∈ s →
+      step s (trm_app val_free (val_loc p)) (Finmap.erase p s) val_unit
+
+/- Multi-step relation -/
+inductive steps : state → trm → state → trm → Prop :=
+  | steps_refl : forall s t,
+      steps s t s t
+  | steps_step : forall s1 s2 s3 t1 t2 t3,
+      step s1 t1 s2 t2 →
+      steps s2 t2 s3 t3 →
+      steps s1 t1 s3 t3
+
+lemma steps_of_step : forall s1 s2 t1 t2,
+  step s1 t1 s2 t2 → steps s1 t1 s2 t2 :=
+by
+  move=> s1 s2 t1 t2 hstep
+  apply steps.steps_step=>//
+
+lemma steps_trans : forall s1 s2 s3 t1 t2 t3,
+  steps s1 t1 s2 t2 →
+  steps s2 t2 s3 t3 →
+  steps s1 t1 s3 t3 :=
+by
+  move=> s1 s2 s3 t1 t2 t3
+  elim=> [s1' s2'| s1' s2' s3' t1' t2' t3' IH1 _ IH3 hstep3]=>//
+
+/- Predicate [reducible s t] for asserting that [(s, t)] can step -/
+def reducible (s : state) (t : trm) : Prop :=
+  exists s' t', step s t s' t'
+
+/- The configuration [(s, t)] is not stuck, i.e. [notstuck s t] if either
+   t is a value or [(s, t)] can step -/
+def notstuck (s : state) (t : trm) : Prop :=
+  trm_is_val t \/ reducible s t
+
+
+/- ------- Big-step Semantics for Primitive Operations ------- -/
+
+/- Big-step relation for unary operators -/
+inductive evalunop : prim → val → (val → Prop) → Prop where
+  | evalunop_neg : forall b1,
+      evalunop val_neg (val_bool b1) (fun v => v = val_bool (¬ b1))
+  | evalunop_opp : forall n1,
+      evalunop val_opp (val_int n1) (fun v => v = val_int (- n1))
+  | evalunop_rand : forall n,
+      n > 0 →
+      evalunop val_rand (val_int n)
+        (fun r => exists n1, r = val_int n1 ∧ 0 <= n1 ∧ n1 < n)
+
+-- def isTrue (p : Prop) : Bool :=
+--   if p then true else false
+
+/- Big-step relation for binary operators -/
+inductive evalbinop : val → val → val → (val->Prop) → Prop where
+
+  /- Since equality of val is not decidable/we don't have a proof of
+     decidability (yet), I will break the rules for equality into their
+     two cases as a temporary solution -/
+  | evalbinop_eq_true : forall v1 v2,
+      v1 = v2 →
+      evalbinop val_eq v1 v2 (fun v => v = val_bool true)
+  | eval_binop_eq_false : forall v1 v2,
+      v1 ≠ v2 →
+      evalbinop val_eq v1 v2 (fun v => v = val_bool false)
+  | evalbinop_neq_true : forall v1 v2,
+      v1 ≠ v2 →
+      evalbinop val_neq v1 v2 (fun v => v = val_bool true)
+  | evalbinop_neq_false : forall v1 v2,
+      v1 = v2 →
+      evalbinop val_neq v1 v2 (fun v => v = val_bool false)
+
+  | evalbinop_add : forall n1 n2,
+      evalbinop val_add (val_int n1) (val_int n2)
+        (fun v => v = val_int (n1 + n2))
+  | evalbinop_sub : forall n1 n2,
+      evalbinop val_sub (val_int n1) (val_int n2)
+        (fun v => v = val_int (n1 - n2))
+  | evalbinop_mul : forall n1 n2,
+      evalbinop val_mul (val_int n1) (val_int n2)
+        (fun v => v = val_int (n1 * n2))
+  | evalbinop_div : forall n1 n2,
+      ¬(n2 = 0) →
+      evalbinop val_div (val_int n1) (val_int n2)
+        (fun v => v = val_int (n1 / n2))
+  | evalbinop_mod : forall n1 n2,
+      ¬(n2 = 0) →
+      evalbinop val_mod (val_int n1) (val_int n2)
+        (fun v => v = val_int (n1 % n2))
+  | evalbinop_le : forall n1 n2,
+      evalbinop val_le (val_int n1) (val_int n2)
+        (fun v => v = val_bool (n1 <= n2))
+  | evalbinop_lt : forall n1 n2,
+      evalbinop val_lt (val_int n1) (val_int n2)
+        (fun v => v = val_bool (n1 < n2))
+  | evalbinop_ge : forall n1 n2,
+      evalbinop val_ge (val_int n1) (val_int n2)
+        (fun v => v = val_bool (n1 >= n2))
+  | evalbinop_gt : forall n1 n2,
+      evalbinop val_gt (val_int n1) (val_int n2)
+        (fun v => v = val_bool (n1 > n2))
+
+  -- Not really sure what's going on in the last rule here since
+  -- in the original CFML code, p2 doesn't have to be a valid pointer (it has
+  -- type int and could be negative), so not sure if this is semantically
+  -- equivalent to what was here before.
+  | evalbinop_ptr_add : forall p1 p2 n,
+      (p2:ℤ) = n + (p1:loc) ->
+      evalbinop val_ptr_add (val_loc p1) (val_int n)
+        (fun v => v = val_loc (Int.toNat p2))
+
+
+/- ---------------- Big-step Semantics -------------------- -/
+
+section eval
+
+/- Predicate for converting predicates [P : val → Prop] into postconditions
+   of type [val → state → Prop] that hold in state s -/
+def purepost (s : state) (P : val → Prop) : val → state → Prop :=
+  fun v s' => P v ∧ s' = s
+
+def purepostin (s : state) (P : val → Prop) (Q : val → state → Prop) : Prop :=
+  -- Equivalent to [purepost S P ===> Q]
+  forall v, P v → Q v s
+
+variable (Q : val → state → Prop)
+
+/- Big-step relation -/
+inductive eval : state → trm → (val → state → Prop) -> Prop where
+  | eval_val : forall s v Q,
+      Q v s ->
+      eval s (trm_val v) Q
+  | eval_fun : forall s x t1 Q,
+      Q (val_fun x t1) s ->
+      eval s (trm_fun x t1) Q
+  | eval_fix : forall s f x t1 Q,
+      Q (val_fix f x t1) s ->
+      eval s (trm_fix f x t1) Q
+  | eval_app_arg1 : forall s1 t1 t2 Q1 Q,
+      ¬ trm_is_val t1 ->
+      eval s1 t1 Q1 ->
+      (forall v1 s2, Q1 v1 s2 -> eval s2 (trm_app v1 t2) Q) ->
+      eval s1 (trm_app t1 t2) Q
+  | eval_app_arg2 : forall s1 v1 t2 Q1 Q,
+      ¬ trm_is_val t2 ->
+      eval s1 t2 Q1 ->
+      (forall v2 s2, Q1 v2 s2 -> eval s2 (trm_app v1 v2) Q) ->
+      eval s1 (trm_app v1 t2) Q
+  | eval_app_fun : forall s1 v1 v2 x t1 Q,
+      v1 = val_fun x t1 ->
+      eval s1 (subst x v2 t1) Q ->
+      eval s1 (trm_app v1 v2) Q
+  | eval_app_fix : forall s v1 v2 f x t1 Q,
+      v1 = val_fix f x t1 ->
+      eval s (subst x v2 (subst f v1 t1)) Q ->
+      eval s (trm_app v1 v2) Q
+  | eval_seq : forall Q1 s t1 t2 Q,
+      eval s t1 Q1 ->
+      (forall v1 s2, Q1 v1 s2 -> eval s2 t2 Q) ->
+      eval s (trm_seq t1 t2) Q
+  | eval_let : forall Q1 s x t1 t2 Q,
+      eval s t1 Q1 ->
+      (forall v1 s2, Q1 v1 s2 -> eval s2 (subst x v1 t2) Q) ->
+      eval s (trm_let x t1 t2) Q
+  | eval_if : forall s (b : Bool) t1 t2 Q,
+      eval s (if b then t1 else t2) Q ->
+      eval s (trm_if (val_bool b) t1 t2) Q
+  | eval_unop : forall op s v1 P Q,
+      evalunop op v1 P ->
+      purepostin s P Q ->
+      eval s (trm_app op v1) Q
+  | eval_binop : forall op s v1 v2 P Q,
+      evalbinop op v1 v2 P ->
+      purepostin s P Q ->
+      eval s (trm_app (trm_app op v1) v2) Q
+  | eval_ref : forall s v Q,
+      v = trm_val v' ->
+      (forall p, ¬ p ∈ s ->
+          Q (val_loc p) (Finmap.insert p v' s)) ->
+      eval s (trm_app val_ref v) Q
+  | eval_get : forall s p Q,
+      p ∈ s ->
+      Q (read_state p s) s ->
+      eval s (trm_app val_get (val_loc p)) Q
+  | eval_set : forall s p v Q,
+      v = trm_val v' ->
+      p ∈ s ->
+      Q val_unit (Finmap.insert p v' s) ->
+      eval s (trm_app (trm_app val_set (val_loc p)) v) Q
+  | eval_free : forall s p Q,
+      p ∈ s ->
+      Q val_unit (Finmap.erase p s) ->
+      eval s (trm_app val_free (val_loc p)) Q
+
+/- Not sure if the rules eval_ref and eval_set are correct. I had to add the
+   condition [v = trm_val v'] to get the definition to type-check. However, this
+   assertion says that the term v is a value but really shouldn't this be
+   that v big-steps to a value? Not sure what the best way to do this is.
+   Perhaps by doing something like the seq rule where there is some
+   intermediate condition Q' for first evaluating v and then composing that
+   with the memory allocation. -/
+
+/- Rule for values to instantiate postconditions -/
+
+lemma eval_val_minimal : forall s v,
+  eval s (trm_val v) (fun v' s' => (v' = v) /\ (s' = s)) :=
+by
+  move=> s v
+  apply eval.eval_val=>//
+
+
+/- Special rules to avoid unecessary use of [evalbinop] and [evalunop] -/
+
+lemma eval_add : forall s n1 n2 Q,
+  Q (val_int (n1 + n2)) s →
+  eval s (trm_app (trm_app val_add (val_int n1)) (val_int n2)) Q :=
+by
+  move=> s n1 n2 Q hQ
+  apply eval.eval_binop
+  { apply evalbinop.evalbinop_add }
+  { move=> v hV =>// }
+
+lemma eval_div : forall s n1 n2 Q,
+  n2 ≠ 0 ->
+  Q (val_int (n1 / n2)) s ->
+  eval s (trm_app (trm_app val_div (val_int n1)) (val_int n2)) Q :=
+by
+  move=> s n1 n2 Q hn2 hQ
+  apply eval.eval_binop
+  { apply evalbinop.evalbinop_div=>// }
+  { move=> v hV =>// }
+
+lemma eval_rand : forall s (n : ℤ) Q,
+  n > 0 ->
+  (forall n1, 0 <= n1 ∧ n1 < n -> Q n1 s) ->
+  eval s (trm_app val_rand (val_int n)) Q :=
+by
+  move=> s n Q hn hn1
+  apply eval.eval_unop
+  { apply evalunop.evalunop_rand=>// }
+  { move=> v hV; cases hV =>// }
+
+
+/- Derived rules for reasoning about applications that don't require checking
+   if terms are already values -/
+
+lemma eval_app_arg1' : forall s1 t1 t2 Q1 Q,
+  eval s1 t1 Q1 ->
+  (forall v1 s2, Q1 v1 s2 -> eval s2 (trm_app v1 t2) Q) ->
+  eval s1 (trm_app t1 t2) Q :=
+by
+  move => s1 t1 t2 Q1 Q hevals1 hevals2
+  sorry
+
+lemma eval_app_arg2' : forall s1 v1 t2 Q1 Q,
+  eval s1 t2 Q1 ->
+  (forall v2 s2, eval s2 (trm_app v1 v2) Q) ->
+  eval s1 (trm_app v1 t2) Q :=
+by
+  sorry
+
+
+/- [eval_like t1 t2] asserts that [t2] evaluates like [t1], i.e.,
+    this relation holds whenever [t2] reduces in small-step to [t1]. -/
+def eval_like (t1 t2:trm) : Prop :=
+  forall s Q, eval s t1 Q -> eval s t2 Q
+
+end eval
